backend/AsmgenproofEFF.v
@@ -447,16 +447,13 @@ Inductive match_states mu: Mach_core -> mem -> Asm_coop.state -> mem -> Prop :=
       match_states mu (Mach_State s fb sp c ms lf) m (State rs tlf) m'
 
   | match_states_init:
-      forall fb m0 m m' f args args' tys retty
+      forall fb m m' f args args' tys retty
         (FIND: Genv.find_funct_ptr ge fb = Some (Internal f))
         (MEXT: Mem.inject (as_inj mu) m m')
         (VINJ: val_list_inject (restrict (as_inj mu) (vis mu)) args args')
         (TYSEQ: sig_args (Mach.fn_sig f) = tys)
         (VALSDEF: val_casted.vals_defined args=true)
         (HASTY: Val.has_type_list args tys)
-        (INITMEM: Genv.init_mem prog = Some m0)
-        (Fwd: Ple (Mem.nextblock m0) (Mem.nextblock m))
-        (Fwd': Ple (Mem.nextblock m0) (Mem.nextblock m'))
         (REP: 4*(2*Zlength args) < Int.max_unsigned),
       match_states mu (Mach_CallstateIn fb args tys retty) m
                       (Asm_CallstateIn fb args' tys retty) m'
@@ -825,15 +822,12 @@ Lemma MATCH_initial: forall v
   (Inj: Mem.inject j m1 m2)
   (VInj: Forall2 (val_inject j) vals1 vals2)
   (PG: meminj_preserves_globals ge j)
-  (R : list_norepet (map fst (prog_defs prog)))
   (J: forall b1 b2 d, j b1 = Some (b2, d) -> 
                       DomS b1 = true /\ DomT b2 = true)
   (RCH: forall b, REACH m2
         (fun b' : Values.block => isGlobalBlock tge b' || getBlocks vals2 b') b =
          true -> DomT b = true)
-  (InitMem : exists m0 : mem, Genv.init_mem prog = Some m0 
-      /\ Ple (Mem.nextblock m0) (Mem.nextblock m1) 
-      /\ Ple (Mem.nextblock m0) (Mem.nextblock m2))
+  (GFI: globalfunction_ptr_inject ge j)
   (GDE: genvs_domain_eq ge tge)
   (HDomS: forall b : Values.block, DomS b = true -> Mem.valid_block m1 b)
   (HDomT: forall b : Values.block, DomT b = true -> Mem.valid_block m2 b),
@@ -927,11 +921,10 @@ Proof. intros.
     as [AA [BB [CC [DD [EE [FF GG]]]]]].
 
   unfold MATCH.
-  destruct InitMem as [m0 [X [Y Z]]].  
   intuition.
 
   rewrite Hsig. 
-  apply match_states_init with (m0 := m0) (f := f); auto.
+  apply match_states_init with (f := f); auto.
   solve[rewrite initial_SM_as_inj; auto].
   rewrite initial_SM_as_inj.
   apply forall_inject_val_list_inject.
@@ -944,14 +937,7 @@ Proof. intros.
   { revert U. simpl. rewrite Hsig. 
     solve[rewrite val_casted.val_has_type_list_func_charact; auto]. }
   rewrite initial_SM_as_inj; auto.
-  red; intros. specialize (Genv.find_funct_ptr_not_fresh prog). intros.
-  specialize (H1 _ _ _ X H). 
-  destruct (valid_init_is_global _ R _ X _ H1) as [id Hid]. 
-  destruct PG as [PGa [PGb PGc]]. split. 
-  solve[rewrite initial_SM_as_inj; eapply PGa; eauto].
-  unfold isGlobalBlock. 
-  apply orb_true_iff. left. apply genv2blocksBool_char1.
-  simpl. exists id; eassumption.
+  rewrite initial_SM_as_inj; auto.
 Qed.
 
 Lemma MATCH_atExternal: forall mu c1 m1 c2 m2 e vals1 ef_sig
@@ -3064,8 +3050,6 @@ Qed.
 
 (** The simulation proof *)
 Theorem transl_program_correct:
-  forall (R: list_norepet (map fst (prog_defs prog)))
-         (init_mem: exists m0, Genv.init_mem prog = Some m0),
   SM_simulation.SM_simulation_inject 
    (Mach_eff_sem hf return_address_offset) (Asm_eff_sem hf) ge tge.
 Proof.
@@ -3086,50 +3070,7 @@ assert (GDE:= GDE_lemma).
 (*MATCH_preserves_globals*)
   apply MATCH_PG.
 (* init*) { intros.
-    eapply (MATCH_initial _ _ _); eauto.
-    destruct init_mem as [m0 INIT].
-    exists m0; split; auto.
-    unfold meminj_preserves_globals in H2.    
-    destruct H2 as [A [B C]].
-
-    assert (P: forall p q, {Ple p q} + {Plt q p}).
-      intros p q.
-      case_eq (Pos.leb p q).
-      intros TRUE.
-      apply Pos.leb_le in TRUE.
-      left; auto.
-      intros FALSE.
-      apply Pos.leb_gt in FALSE.
-      right; auto.
-
-    cut (forall b, Plt b (Mem.nextblock m0) -> 
-           exists id, Genv.find_symbol ge id = Some b). intro D.
-    
-    split.
-    destruct (P (Mem.nextblock m0) (Mem.nextblock m1)); auto.
-    exfalso. 
-    destruct (D _ p).
-    apply A in H2.
-    assert (Mem.valid_block m1 (Mem.nextblock m1)).
-      eapply Mem.valid_block_inject_1; eauto.
-    clear - H7; unfold Mem.valid_block in H7.
-    xomega.
-
-    destruct (P (Mem.nextblock m0) (Mem.nextblock m2)); auto.
-    exfalso. 
-    destruct (D _ p).
-    apply A in H2.
-    assert (Mem.valid_block m2 (Mem.nextblock m2)).
-      eapply Mem.valid_block_inject_2; eauto.
-    clear - H7; unfold Mem.valid_block in H7.
-    xomega.
-    
-    intros b LT.    
-    unfold ge. 
-    apply valid_init_is_global with (b0 := b) in INIT.
-    eapply INIT; auto.
-    apply R.
-    apply LT. } 
+    eapply (MATCH_initial _ _ _); eauto. }
 { (* halted *)
     intros. destruct H as [MC [RC [PG [Glob [VAL [WD INJ]]]]]].
     inv MC; try solve[inv H0]. simpl in H0.
